src/medium.lean
@@ -1,29 +1,36 @@
 
 import tactic
 import logic.basic
+import category.liftable
+import liftable
 
-universes u
+universes u v
 
-inductive put_m_intl (α : Type u)
-| pure : α → put_m_intl
-| write : unsigned → (unit → put_m_intl) → put_m_intl
+inductive put_m' (α : Type u)
+| pure : α → put_m'
+| write : unsigned → (unit → put_m') → put_m'
 
-def put_m_intl.bind {α β} : put_m_intl α → (α → put_m_intl β) → put_m_intl β
-| (put_m_intl.pure x)   f := f x
-| (put_m_intl.write w f) g := put_m_intl.write w $ λ u, put_m_intl.bind (f u) g
+def put_m'.bind {α β} : put_m' α → (α → put_m' β) → put_m' β
+| (put_m'.pure x)   f := f x
+| (put_m'.write w f) g := put_m'.write w $ λ u, put_m'.bind (f u) g
 
-instance : monad put_m_intl :=
-{ pure := λ α, put_m_intl.pure
-, bind := @put_m_intl.bind }
+instance : monad put_m' :=
+{ pure := λ α, put_m'.pure
+, bind := @put_m'.bind }
 
-instance : is_lawful_monad put_m_intl :=
-sorry
+instance : is_lawful_monad put_m' :=
+by { refine { .. }; intros;
+       try { refl };
+       induction x;
+       try { refl };
+     { dsimp [put_m'.bind] at *, congr, simp * } }
 
-def put_m := put_m_intl punit
+@[reducible]
+def put_m := put_m' punit
 
 def put_m.eval : put_m → list unsigned
-| (put_m_intl.pure x) := []
-| (put_m_intl.write w f) := w :: put_m.eval (f punit.star)
+| (put_m'.pure x) := []
+| (put_m'.write w f) := w :: put_m.eval (f punit.star)
 
 inductive get_m : Type u → Type (u+1)
 | fail {α} : get_m α
@@ -37,12 +44,70 @@ def get_m.bind : Π {α β}, get_m α → (α → get_m β) → get_m β
 | _ _ (get_m.read f) g := get_m.read $ λ w, get_m.bind (f w) g
 | _ _ (get_m.loop x₀ f g) h := get_m.loop x₀ f (λ r, get_m.bind (g r) h)
 
+
+def get_m.map : Π {α β : Type u}, (α → β) → get_m α → get_m β
+| _ _ _ (get_m.fail) := get_m.fail
+| _ _ f (get_m.pure x) := get_m.pure $ f x
+| _ _ f (get_m.read g) := get_m.read $ λ w, get_m.map f (g w)
+| _ _ h (get_m.loop x₀ f g) := get_m.loop x₀ f (λ r, get_m.map h (g r))
+
+instance : functor get_m.{u} :=
+{ map := @get_m.map }
+
+def get_m.seq {α β : Type u} : Π (f : get_m (α → β)) (x : get_m α), get_m β :=
+λ (f : get_m (α → β)) (x : get_m α), get_m.bind f (λ f, f <$> x)
+
+instance : applicative get_m :=
+{ to_functor := get_m.functor
+, pure := λ α, get_m.pure
+, seq := @get_m.seq }
+open function
+
+
+-- lemma get_m.seq_assoc {α β γ : Type u} (x : get_m α) (g : get_m (α → β)) (h : get_m (β → γ)) :
+--   h <*> (g <*> x) = (@comp α β γ <$> h) <*> g <*> x :=
+-- begin
+--   refine get_m.rec_on h _ _ _ _; intros; dsimp [(<*>),(<$>),get_m.seq,get_m.bind],
+--   erw get_m.bind,
+--   change get_m.fail = _,
+--   refl, dunfold get_m.bind,
+-- end
+
+instance : is_lawful_functor get_m :=
+sorry
+-- by { constructor; intros;
+--      dsimp [(<$>),get_m.seq];
+--      induction x;
+--      try { refl };
+--      simp [get_m.bind,get_m.seq,*]; ext, rw x_ih, }
+
+instance : is_lawful_applicative get_m :=
+sorry
+-- by { constructor; intros; dsimp [(<*>),pure,(<$>),get_m.seq]; try { refl },
+--        -- refl },
+--      simp [get_m.bind],
+--      induction g generalizing h x, simp [get_m.bind,(∘)], refl,
+--      }
+
 instance : monad get_m :=
-{ pure := λ α, get_m.pure
+{ to_applicative := get_m.applicative
 , bind := @get_m.bind }
 
 instance : is_lawful_monad get_m :=
 sorry
+-- { is_lawful_monad . bind_assoc := by { intros, dsimp, refl },
+--   pure_bind := by { intros, dsimp, refl },
+--   bind_pure_comp_eq_map := by { intros, dsimp, refl },
+--   bind_map_eq_seq := by { intros, dsimp, refl },
+--   pure_seq_eq_map := by { intros, dsimp, refl },
+--   map_pure := by { intros, dsimp, refl },
+--   seq_pure := by { intros, dsimp, refl },
+--   seq_assoc := by { intros, dsimp, refl } }
+-- by { constructor; intros; dsimp [(>>=)],
+--      refl,
+--      induction x; try { refl };
+--      dsimp [(>>=),get_m.bind];
+--      try { refl }; congr; simp * }
 
 def get_m.eval {α} : list unsigned → get_m α → option α
 | [] (get_m.pure x) := pure x
@@ -59,10 +124,10 @@ def get_m.eval {α} : list unsigned → get_m α → option α
 
 
 def read_write : Π {α}, get_m α → put_m → option α
-| ._ (get_m.pure x) (put_m_intl.pure _) := some x
-| _ _ (put_m_intl.pure _) := none
-| ._ (get_m.read f) (put_m_intl.write w g) := read_write (f w) (g punit.star)
-| _ (@get_m.loop α β γ x₀ f g) (put_m_intl.write w h) :=
+| ._ (get_m.pure x) (put_m'.pure _) := some x
+| _ _ (put_m'.pure _) := none
+| ._ (get_m.read f) (put_m'.write w g) := read_write (f w) (g punit.star)
+| _ (@get_m.loop α β γ x₀ f g) (put_m'.write w h) :=
   read_write
     (do r ← f x₀ w,
        match r with
@@ -70,11 +135,11 @@ def read_write : Π {α}, get_m α → put_m → option α
        | (sum.inl r) := g r
        end )
     (h punit.star)
-| _ _ (put_m_intl.write w g) := none
+| _ _ (put_m'.write w g) := none
 
 def read_write' : Π {α}, get_m α → put_m → option (α × put_m)
-| _ (get_m.read f) (put_m_intl.write w g) := read_write' (f w) (g punit.star)
-| _ (@get_m.loop α β γ x₀ f g) (put_m_intl.write w h) :=
+| _ (get_m.read f) (put_m'.write w g) := read_write' (f w) (g punit.star)
+| _ (@get_m.loop α β γ x₀ f g) (put_m'.write w h) :=
   read_write'
     (do r ← f x₀ w,
        match r with
@@ -82,10 +147,10 @@ def read_write' : Π {α}, get_m α → put_m → option (α × put_m)
        | (sum.inl r) := g r
        end )
     (h punit.star)
--- | _ (get_m.pure x) m@(put_m_intl.write w g) := some (x,m)
+-- | _ (get_m.pure x) m@(put_m'.write w g) := some (x,m)
 | _ (get_m.pure x) m := some (x,m)
-| _ _ (put_m_intl.pure _) := none
-| _ (get_m.fail) (put_m_intl.write _ _) := none
+| _ _ (put_m'.pure _) := none
+| _ (get_m.fail) (put_m'.write _ _) := none
 -- | _ _ m := none
 
 lemma read_read_write_write {α} (x : get_m α) (m : put_m) (i : α) :
@@ -111,22 +176,22 @@ by cases x; refl
 -- | read_write {α} (x : α) (w : unsigned)
 --   (f : unsigned → get_m α) (g : punit → put_m) (m : put_m) :
 --   agree x (f w) (g punit.star) m →
---   agree x (get_m.read f) (put_m_intl.write w g) m
+--   agree x (get_m.read f) (put_m'.write w g) m
 -- | loop_write {α} (x : α) {β γ} (σ₀ σ₁ : β) (w : unsigned)
 --   (f : β → unsigned → get_m (γ ⊕ β)) (f' : γ → get_m α)
 --   (g : punit → put_m) (m m' : put_m) :
 --   agree (sum.inr σ₁) (f σ₀ w) (g punit.star) m' →
 --   agree x (get_m.loop σ₁ f f') m' m →
---   agree x (get_m.loop σ₀ f f') (put_m_intl.write w g) m
+--   agree x (get_m.loop σ₀ f f') (put_m'.write w g) m
 -- | loop_exit_write {α} (x : α) {β γ} (σ₀ : β) (r : γ) (w : unsigned)
 --   (f : β → unsigned → get_m (γ ⊕ β)) (f' : γ → get_m α)
 --   (g : punit → put_m) (m m' : put_m) :
 --   agree (sum.inl r) (f σ₀ w) (g punit.star) m' →
 --   agree x (f' r) m' m →
---   agree x (get_m.loop σ₀ f f') (put_m_intl.write w g) m
+--   agree x (get_m.loop σ₀ f f') (put_m'.write w g) m
 
 -- lemma agree_spec {α} (g : get_m α) (m : put_m) (x : α) :
---   agree x g m (put_m_intl.pure punit.star) ↔ g -<< m = some x :=
+--   agree x g m (put_m'.pure punit.star) ↔ g -<< m = some x :=
 -- begin
 --   split; intro h,
 --   { cases h,
@@ -141,7 +206,7 @@ lemma read_write_loop_bind {α β γ φ : Type u} (i : α)
       (body : α → unsigned → get_m (φ ⊕ α))
       (f₀ : φ → get_m β) (f₁ : β → get_m γ)
       (m : punit → put_m) (w : unsigned) :
-  (get_m.loop i body f₀ >>= f₁) -<<< put_m_intl.write w m =
+  (get_m.loop i body f₀ >>= f₁) -<<< put_m'.write w m =
   (body i w >>= read_write'._match_1 _ _ _ body f₀ >>= f₁) -<<< m punit.star :=
 begin
   rw bind_assoc,
@@ -168,12 +233,20 @@ lemma read_write_left_overs_bind {α} (f : punit → put_m) (i : α)
   x₀ -<<< x₁ = some (i,x₂) → x₀ -<<< (x₁ >>= f) = some (i,x₂ >>= f) :=
 begin
   induction x₁ generalizing x₀ x₂,
-  cases x₀; simp [(>>=),put_m_intl.bind,read_write',pure_read_write],
+  cases x₀; simp [(>>=),put_m'.bind,read_write',pure_read_write],
   { intros, subst x₂, tauto },
-  cases x₀; simp [(>>=),put_m_intl.bind,read_write'],
+  cases x₀; simp [(>>=),put_m'.bind,read_write'],
   { intros, substs x₂ i, split; refl },
   { apply x₁_ih, },
   { apply x₁_ih, },
+end
+
+lemma option_eq_forall_some {α} (x y : option α) :
+  x = y ↔ ∀ z, x = some z ↔ y = some z :=
+begin
+  split; intro h, { rw h; intro, refl },
+  { cases y, cases x, refl,
+    symmetry, rw ← h, rw h, },
 end
 
 lemma read_write_weakening {α}
@@ -181,9 +254,7 @@ lemma read_write_weakening {α}
   (h : y₀ -<<< x₀ = y₁ -<<< x₁) :
   y₀ -<< x₀ = y₁ -<< x₁ :=
 begin
-  suffices : ∀ z, y₀ -<< x₀ = some z ↔ y₁ -<< x₁ = some z,
-  { cases y₁ -<< x₁, cases y₀ -<< x₀, refl,
-    symmetry, rw ← this, rw this, },
+  rw option_eq_forall_some,
   intro, simp [read_read_write_write,h],
 end
 
@@ -224,4 +295,137 @@ begin
   induction x₁ generalizing x₀; cases x₀; try { refl },
   simp! [*,read_write],
   simp! [*,read_write], refl,
+end
+open ulift
+
+lemma get_m.fold_bind {α β} (x : get_m α) (f : α → get_m β) :
+  get_m.bind x f = x >>= f := rfl
+
+lemma map_read_write {α β} (f : α → β) (x : get_m α) (y : put_m) :
+  (f <$> x) -<< y = f <$> (x -<< y) :=
+begin
+  rw [← bind_pure_comp_eq_map,← bind_pure_comp_eq_map],
+  symmetry,
+  simp [(>>=)],
+  induction y generalizing x,
+  { cases x; refl },
+  { cases x; simp [read_write]; try { refl };
+    simp [get_m.bind,read_write,y_ih],
+    congr' 1, cases h : x_a_1 x_a y_a, refl,
+    cases a; refl,
+    dsimp [(>>=),get_m.bind],
+    congr, ext, simp [get_m.fold_bind],
+    rw bind_assoc, congr, ext z, cases z; refl,
+    simp [get_m.fold_bind], rw bind_assoc, congr, ext x,
+    cases x; refl, }
+end
+
+def sum_ulift (α β : Type u) : (α ⊕ β) ≃ (ulift.{v} α ⊕ ulift.{v} β) :=
+(equiv.sum_congr equiv.ulift.symm equiv.ulift.symm)
+
+-- def get_m.up : Π {α : Type u} {β : Type.{max u v}} (Heq : α ≃ β), get_m α → get_m β
+-- | _ _ Heq (get_m.pure x) := get_m.pure $ Heq x
+-- | _ _ Heq (get_m.fail) := get_m.fail
+-- | _ _ Heq (get_m.read f) := get_m.read (λ w, get_m.up Heq (f w))
+-- | _ β' Heq (@get_m.loop α β γ x f g) :=
+--   get_m.loop (up.{v} x)
+--     (λ a b, get_m.up (sum_ulift α β) (f (down.{v} a) b))
+--     (λ w, get_m.up Heq (g $ down w))
+
+def get_m.up : Π {α : Type u} {β : Type.{max u v}} (Heq : α → β), get_m α → get_m β :=
+λ α β f x, (@get_m.rec_on (λ α _, Π β, (α → β) → get_m β) α x
+(λ α β f, get_m.fail)
+(λ α x β f, get_m.pure $ f x)
+(λ α next get_m_up β f, get_m.read $ λ w, get_m_up w _ f)
+(λ α β γ x₀ body rest get_m_up₀ get_m_up₁ β' f,
+  get_m.loop (up x₀)
+    (λ a b, get_m_up₀ (down a) b (ulift.{v} α ⊕ ulift.{v} β)
+                      (sum_ulift α β))
+    (λ r, get_m_up₁ (down r) _ f) )) β f
+
+section eqns
+
+variables {α β' γ : Type u} {β : Type.{max u v}} (Heq : α → β) (x : get_m α)
+
+variables {i : α} {f : unsigned → get_m α}
+variables {f' : β' → unsigned → get_m (γ ⊕ β')}
+variables {g' : γ → get_m α} {j : β'}
+
+@[simp] lemma get_m.up.eqn_1 : get_m.up Heq (get_m.pure i) = get_m.pure (Heq i) := rfl
+@[simp] lemma get_m.up.eqn_2 : get_m.up Heq (get_m.fail) = get_m.fail := rfl
+@[simp] lemma get_m.up.eqn_3 : get_m.up Heq (get_m.read f) = get_m.read (λ w, get_m.up Heq (f w)) := rfl
+@[simp] lemma get_m.up.eqn_4 :
+  get_m.up Heq (get_m.loop j f' g') =
+  get_m.loop (up.{v} j)
+    (λ a b, get_m.up (sum_ulift γ β') (f' (down.{v} a) b))
+    (λ w, get_m.up Heq (g' $ down w)) := rfl
+
+end eqns
+
+def put_m.up {α : Type u} {β : Type v} (Heq : α → β) : put_m' α → put_m' β
+| (put_m'.pure x) := put_m'.pure $ Heq x
+| (put_m'.write w f) := put_m'.write w $ λ u, put_m.up $ f u
+
+instance : liftable1 put_m'.{u} put_m'.{v} :=
+{ up := λ α β (eq : α ≃ β) x, put_m.up eq x
+, down := λ α β (eq : α ≃ β) x, put_m.up eq.symm x
+, down_up := by intros; induction x; simp [put_m.up,*]
+, up_down := by intros; induction x; simp [put_m.up,*]  }
+
+open pliftable (up')
+
+lemma up_bind {α β : Type u} {β' : Type (max u v)} (x : get_m α) (g : α → get_m β) (f : β → β') :
+  (x >>= g).up f = x.up up.{v} >>= (λ i : ulift α, (g $ down i).up f) :=
+begin
+  dsimp [(>>=)],
+  induction x generalizing f g; try { refl };
+    simp [get_m.bind,*]
+end
+
+lemma equiv_bind {m} [monad m] [is_lawful_monad m] {α α' β}
+  (Heq : α ≃ α') (x : m α) (f : α → m β) :
+  x >>= f = (Heq <$> x) >>= f ∘ Heq.symm :=
+sorry
+
+def sum.map {α α' β β'} (f : α → α') (g : β → β') : α ⊕ β → α' ⊕ β'
+| (sum.inr x) := sum.inr $ g x
+| (sum.inl x) := sum.inl $ f x
+
+def equiv.ulift_sum {α β} : (ulift $ α ⊕ β) ≃ (ulift α ⊕ ulift β) :=
+{ to_fun := λ x, sum.map up up (down x),
+  inv_fun := λ x, up $ sum.map down down x,
+  right_inv := by intro; casesm* [_ ⊕ _,ulift _]; refl,
+  left_inv := by intro; casesm* [_ ⊕ _,ulift _]; refl }
+
+lemma map_get_m_up {α : Type u} {β γ} (x : get_m α) (f : α → β) (g : β → γ) :
+  g <$> get_m.up f x = get_m.up (g ∘ f) x :=
+begin
+  dsimp [(<$>)],
+  induction x; simp [get_m.map,*]; refl,
+end
+
+lemma up_read_write {α : Type u} {α' : Type (max u v)} (x : get_m α) (y : put_m) (f : α ≃ α') :
+  x.up f -<< up' y = liftable1.up f (x -<< y) :=
+begin
+  dsimp [up',liftable1.up],
+  induction y generalizing x f,
+  cases x; simp; refl,
+  cases x; simp [up',liftable.up',liftable1.up,read_write,put_m.up,*], refl, refl, refl,
+  rw [read_write,← y_ih,up_bind],
+    apply congr,
+    { apply congr_arg, rw equiv_bind (@equiv.ulift_sum.{u u v v v} x_α x_β) ,
+      congr,
+      { rw map_get_m_up, congr, ext, cases x; refl },
+      simp [(∘)], ext, cases x;
+      dsimp [read_write._match_1,equiv.ulift_sum,sum.map], refl,
+      cases x, refl, apply_instance },
+    congr,
+end
+
+lemma up_read_write' {α : Type u} {α' : Type (max u v)}
+  {x : get_m α} {y : put_m} (f : α → α') (f' : α ≃ α')
+  (h : ∀ i, f i = f' i) :
+  x.up f -<< up' y = liftable1.up f' (x -<< y) :=
+begin
+  rw ← up_read_write, congr, ext, apply h
 end
