src/category/serial.lean
@@ -1,0 +1,9 @@
+
+import tactic
+
+@[simp]
+lemma bind_pure_star {m} [monad m] [is_lawful_monad m] (x : m punit) :
+  x >>= (λ (_x : punit), pure punit.star : punit → m punit) = x :=
+by { transitivity,
+     { apply congr_arg, ext z, cases z, refl },
+     { simp } }
